split extension_safety into a new file

compositional_compcert/extension.v
@@ -70,211 +70,6 @@ End Extension. End Extension.
 Implicit Arguments Extension.Sig [M G D xT].
 Implicit Arguments Extension.Make [G xT cT M D Z Zint Zext].
 
-(** * Safe Extensions *)
-
-Section SafeExtension. Variables
- (M: Type) (** memories *)
- (Z: Type) (** external states *)
- (Zint: Type) (** portion of Z implemented by extension *)
- (Zext: Type) (** portion of Z external to extension *)
- (G: Type) (** global environments of extended semantics *)
- (D: Type) (** extension initialization data *)
- (xT: Type) (** corestates of extended semantics *)
- (esem: CoreSemantics G xT M D) (** extended semantics *)
- (esig: ef_ext_spec M Zext) (** extension signature *)
- (gT: nat -> Type) (** global environments of core semantics *)
- (dT: nat -> Type) (** initialization data *)
- (cT: nat -> Type) (** corestates of core semantics *)
- (csem: forall i:nat, CoreSemantics (gT i) (cT i) M (dT i)) (** a set of core semantics *)
- (csig: ef_ext_spec M Z). (** client signature *)
-
- Variables (ge: G) (genv_map : forall i:nat, gT i).
-
- Import Extension.
-
- Definition all_safe (E: Sig Z Zint Zext esem esig gT dT cT csem csig)
-   (n: nat) (z: Z) (w: xT) (m: M) :=
-  forall i c, proj_core E i w = Some c -> 
-  safeN (csem i) csig (genv_map i) n z c m.
-
- Definition safe_extension (E: Sig Z Zint Zext esem esig gT dT cT csem csig) :=
-  forall n s m z, all_safe E n (zmult E (proj_zint E s) z) s m -> 
-  safeN esem (link_ext_spec (handled E) esig) ge n z s m.
-
-End SafeExtension.
-
-Module SafetyInvariant. Section SafetyInvariant. Variables
- (M: Type) (** memories *)
- (Z: Type) (** external states *)
- (Zint: Type) (** portion of Z implemented by extension *)
- (Zext: Type) (** portion of Z external to extension *)
- (G: Type) (** global environments of extended semantics *)
- (D: Type) (** extension initialization data *)
- (xT: Type) (** corestates of extended semantics *)
- (esem: CoreSemantics G xT M D) (** extended semantics *)
- (esig: ef_ext_spec M Zext) (** extension signature *)
- (gT: nat -> Type) (** global environments of core semantics *)
- (dT: nat -> Type) (** initialization data *)
- (cT: nat -> Type) (** corestates of core semantics *)
- (csem: forall i:nat, CoreSemantics (gT i) (cT i) M (dT i)) (** a set of core semantics *)
- (csig: ef_ext_spec M Z). (** client signature *)
-
- Variables (ge: G) (genv_map : forall i:nat, gT i).
- Variable E: Extension.Sig Z Zint Zext esem esig gT dT cT csem csig.
-
-Definition proj_zint := E.(Extension.proj_zint). 
-Coercion proj_zint : xT >-> Zint.
-
-Definition proj_zext := E.(Extension.proj_zext).
-Coercion proj_zext : Z >-> Zext.
-
-Notation ALL_SAFE := (all_safe genv_map E). 
-Notation PROJ_CORE := E.(Extension.proj_core).
-Notation "zint \o zext" := (E.(Extension.zmult) zint zext) 
-  (at level 66, left associativity). 
-Notation ACTIVE := (E.(Extension.active)).
-Notation active_proj_core := E.(Extension.active_proj_core).
-Notation zint_invar_after_external := E.(Extension.zint_invar_after_external).
-
-Inductive safety_invariant: Type := SafetyInvariant: forall 
- (** Coresteps preserve the all-safety invariant. *)
- (core_pres: forall n z (s: xT) c m s' c' m', 
-   ALL_SAFE (S n) (s \o z) s m -> 
-   PROJ_CORE (ACTIVE s) s = Some c -> 
-   corestep (csem (ACTIVE s)) (genv_map (ACTIVE s)) c m c' m' -> 
-   corestep esem ge s m s' m' -> 
-   ALL_SAFE n (s' \o z) s' m')
-
- (** Corestates satisfying the invariant can corestep. *)
- (core_prog: forall n z s m (c: cT (ACTIVE s)),
-   ALL_SAFE (S n) z s m -> 
-   PROJ_CORE (ACTIVE s) s = Some c -> 
-   runnable (csem (ACTIVE s)) c=true -> 
-   exists c', exists s', exists m', 
-    corestep (csem (ACTIVE s)) (genv_map (ACTIVE s)) c m c' m' /\ 
-    corestep esem ge s m s' m' /\
-    PROJ_CORE (ACTIVE s) s' = Some c')
-
- (** "Handled" steps respect function specifications. *)
- (handled_pres: forall s z m (c: cT (ACTIVE s)) s' m' 
-     (c': cT (ACTIVE s)) ef sig args P Q x, 
-  let i := ACTIVE s in PROJ_CORE i s = Some c -> 
-   at_external (csem i) c = Some (ef, sig, args) -> 
-   Extension.handled E ef -> 
-   spec_of ef csig = (P, Q) -> 
-   P x (sig_args sig) args (s \o z) m -> 
-   corestep esem ge s m s' m' -> 
-   PROJ_CORE i s' = Some c' -> 
-    ((at_external (csem i) c' = Some (ef, sig, args) /\ 
-      P x (sig_args sig) args (s' \o z) m' /\ i <> ACTIVE s') \/
-    (exists ret, after_external (csem i) ret c = Some c' /\ 
-      Q x (sig_res sig) ret (s' \o z) m')))
-
- (** "Handled" states satisfying the invariant can step or are safely halted;
-    core states that remain "at_external" over handled steps are unchanged. *)
- (handled_prog: forall n (z: Zext) (s: xT) m c,
-   ALL_SAFE (S n) (s \o z) s m -> 
-   PROJ_CORE (ACTIVE s) s = Some c -> 
-   runnable (csem (ACTIVE s)) c=false -> 
-   at_external esem s = None -> 
-   (exists s', exists m', corestep esem ge s m s' m' /\ 
-     forall i c, PROJ_CORE i s = Some c -> 
-       exists c', PROJ_CORE i s' = Some c' /\
-        (forall ef args ef' args', 
-          at_external (csem i) c = Some (ef, args) -> 
-          at_external (csem i) c' = Some (ef', args') -> c=c')) \/
-   (exists rv, safely_halted esem s = Some rv))
-
- (** Safely halted threads remain halted. *)
- (safely_halted_halted: forall s m s' m' i c rv,
-   PROJ_CORE i s = Some c -> 
-   safely_halted (csem i) c = Some rv -> 
-   corestep esem ge s m s' m' -> PROJ_CORE i s' = Some c)
-
- (** Safety of other threads is preserved when handling one step of blocked
-    thread [i]. *)
- (handled_rest: forall s m s' m' c,
-   PROJ_CORE (ACTIVE s) s = Some c -> 
-   ((exists ef, exists sig, exists args, 
-      at_external (csem (ACTIVE s)) c = Some (ef, sig, args)) \/ 
-     exists rv, safely_halted (csem (ACTIVE s)) c = Some rv) -> 
-   at_external esem s = None -> 
-   corestep esem ge s m s' m' -> 
-   (forall j c0, ACTIVE s <> j ->  
-    (PROJ_CORE j s' = Some c0 -> PROJ_CORE j s = Some c0) /\
-    (forall n z z', PROJ_CORE j s = Some c0 -> 
-      safeN (csem j) csig (genv_map j) (S n) (s \o z) c0 m -> 
-      safeN (csem j) csig (genv_map j) n (s' \o z') c0 m')))
-
- (** If the extended machine is at external, then the active thread is at
-    external (an extension only implements external functions, it doesn't
-    introduce them). *)
- (at_extern_call: forall s ef sig args,
-   at_external esem s = Some (ef, sig, args) -> 
-   exists c, PROJ_CORE (ACTIVE s) s = Some c /\
-    at_external (csem (ACTIVE s)) c = Some (ef, sig, args))
-
- (** Inject the results of an external call into the extended machine state. *)
- (at_extern_ret: forall z s (c: cT (ACTIVE s)) m z' m' tys args ty ret c' ef sig x 
-    (P: ext_spec_type esig ef -> list typ -> list val -> Zext -> M -> Prop) 
-    (Q: ext_spec_type esig ef -> option typ -> option val -> Zext -> M -> Prop),
-   PROJ_CORE (ACTIVE s) s = Some c -> 
-   at_external esem s = Some (ef, sig, args) -> 
-   spec_of ef esig = (P, Q) -> 
-   P x tys args (s \o z) m -> Q x ty ret z' m' -> 
-   after_external (csem (ACTIVE s)) ret c = Some c' -> 
-   exists s': xT, 
-    z' = s' \o z' /\
-    after_external esem ret s = Some s' /\ 
-    PROJ_CORE (ACTIVE s) s' = Some c')
-
- (** Safety of other threads is preserved when returning from an external 
-    function call. *)
- (at_extern_rest: forall z s (c: cT (ACTIVE s)) m z' s' m' tys args ty ret c' ef x sig
-    (P: ext_spec_type esig ef -> list typ -> list val -> Zext -> M -> Prop) 
-    (Q: ext_spec_type esig ef -> option typ -> option val -> Zext -> M -> Prop),
-   PROJ_CORE (ACTIVE s) s = Some c -> 
-   at_external esem s = Some (ef, sig, args) -> 
-   spec_of ef esig = (P, Q) -> 
-   P x tys args (s \o z) m -> Q x ty ret z' m' -> 
-   after_external (csem (ACTIVE s)) ret c = Some c' -> 
-   after_external esem ret s = Some s' -> 
-   PROJ_CORE (ACTIVE s) s' = Some c' ->  
-   (forall j (CS0: CoreSemantics (gT j) (cT j) M (dT j)) c0, ACTIVE s <> j -> 
-    (PROJ_CORE j s' = Some c0 -> PROJ_CORE j s = Some c0) /\
-    (forall ge n, PROJ_CORE j s = Some c0 -> 
-      safeN CS0 csig ge (S n) (s \o z) c0 m -> 
-      safeN CS0 csig ge n (s' \o z') c0 m'))),
- safety_invariant.
-
-End SafetyInvariant. End SafetyInvariant.
-
-Module EXTENSION_SAFETY. Section EXTENSION_SAFETY. Variables
- (M: Type) (** memories *)
- (Z: Type) (** external states *)
- (Zint: Type) (** portion of Z implemented by extension *)
- (Zext: Type) (** portion of Z external to extension *)
- (G: Type) (** global environments of extended semantics *)
- (D: Type) (** extension initialization data *)
- (xT: Type) (** corestates of extended semantics *)
- (esem: CoreSemantics G xT M D) (** extended semantics *)
- (esig: ef_ext_spec M Zext) (** extension signature *)
- (gT: nat -> Type) (** global environments of core semantics *)
- (dT: nat -> Type) (** initialization data *)
- (cT: nat -> Type) (** corestates of core semantics *)
- (csem: forall i:nat, CoreSemantics (gT i) (cT i) M (dT i)) (** a set of core semantics *)
- (csig: ef_ext_spec M Z). (** client signature *)
-
- Variables (ge: G) (genv_map : forall i:nat, gT i).
- Variable E: Extension.Sig Z Zint Zext esem esig gT dT cT csem csig.
-
-Import SafetyInvariant.
-
-Record Sig := Make {_: safety_invariant ge genv_map E -> 
-                       safe_extension ge genv_map E}.
-
-End EXTENSION_SAFETY. End EXTENSION_SAFETY.
-
 (** Some administrative requirements on the interactions between extensions and
    inner cores. Perhaps some of these conditions could be merged with those for
    "safe" extensions. *)
@@ -298,9 +93,9 @@ Section CoreCompatible. Variables
  Variables (ge: G) (genv_map : forall i:nat, gT i).
  Variable E: Extension.Sig Z Zint Zext esem esig gT dT cT csem csig.
 
-Import Extension.
+ Import Extension.
 
-Inductive core_compatible: Type := CoreCompatible: forall
+ Inductive core_compatible: Type := CoreCompatible: forall
  (** When the active thread is runnable, a step in the extended semantics can be
     tracked back to a corestep of the active thread. *)
  (runnable_corestep: forall s m s' m' c,
@@ -311,7 +106,13 @@ Inductive core_compatible: Type := CoreCompatible: forall
     proj_core E (active E s) s' = Some c') 
 
  (** After a corestep of the active inner core, the active thread's new
-    corestate is appropriately injected into the extended state. *)
+    corestate is appropriately injected into the extended state. Note that 
+    this condition typically imposes determinism on the inner core semantics. 
+    We can live with this because we are in general dealing with deterministic 
+    semantics.  To weaken the determinism condition, one could make proj_core 
+    a relation, or equivalently, have proj_core project a /set/ of corestates; 
+    but at the current stage, the conveniences of proj_core-as-function appear to 
+    outweigh the disadvantages. *)
  (corestep_pres: forall s (c: cT (active E s)) m c' s' m',
    proj_core E (active E s) s = Some c -> 
    corestep (csem (active E s)) (genv_map (active E s)) c m c' m' -> 
@@ -319,8 +120,8 @@ Inductive core_compatible: Type := CoreCompatible: forall
    active E s = active E s' /\ 
    proj_core E (active E s) s' = Some c')
 
- (** A corestep of the currently active core forces a corestep of the extended
-    semantics*)
+ (** A corestep of the currently active core forces a corestep of the 
+    extended semantics *)
  (corestep_prog: forall s (c: cT (active E s)) m c' m',
    proj_core E (active E s) s = Some c -> 
    corestep (csem (active E s)) (genv_map (active E s)) c m c' m' -> 
@@ -346,8 +147,8 @@ Inductive core_compatible: Type := CoreCompatible: forall
    after_external esem retv s = Some s' -> 
    active E s=active E s')
 
- (** Extension states can be updated to match after_external on the active
-    core. *)
+ (** Extension states can be updated to match after_external on the 
+    active core. *)
  (after_ext_prog: forall s (c: cT (active E s)) c' retv,
    proj_core E (active E s) s = Some c -> 
    after_external (csem (active E s)) retv c = Some c' -> 
@@ -361,8 +162,7 @@ Inductive core_compatible: Type := CoreCompatible: forall
    forall j, (active E s)<>j -> 
     proj_core E j s = proj_core E j s')
 
- (** Hypothesis repeated from extension signature to get around a bug in
- [Program]. *)
+ (*Hypothesis repeated from extension signature to get around a bug in [Program]*)
  (at_extern_call: forall s ef sig args,
    at_external esem s = Some (ef, sig, args) -> 
    exists c, proj_core E (active E s) s = Some c /\
