compositional_compcert/extension_proof.v
@@ -6,6 +6,7 @@ Require Import compositional_compcert.rg_forward_simulations.
 Require Import compositional_compcert.step_lemmas. 
 Require Import compositional_compcert.extspec. 
 Require Import compositional_compcert.extension.
+Require Import compositional_compcert.extension_safety.
 Require Import compositional_compcert.extension_simulations.
 Require Import compositional_compcert.Coqlib2.
 Require Import compositional_compcert.wf_lemmas.
